ModalLogic/complete/Canonical_Kripke.v
@@ -1,0 +1,129 @@
+Require Import Coq.Logic.FunctionalExtensionality.
+Require Import Coq.Logic.Classical_Prop.
+Require Import Coq.Logic.Classical_Pred_Type.
+Require Import Logic.lib.Bijection.
+Require Import Logic.lib.Countable.
+Require Import Logic.GeneralLogic.Base.
+Require Import Logic.GeneralLogic.KripkeModel.
+Require Import Logic.GeneralLogic.ProofTheory.BasicSequentCalculus.
+Require Import Logic.GeneralLogic.Semantics.Kripke.
+Require Import Logic.GeneralLogic.Complete.ContextProperty.
+Require Import Logic.GeneralLogic.Complete.ContextProperty_Kripke.
+Require Import Logic.GeneralLogic.Complete.Lindenbaum.
+Require Import Logic.MinimunLogic.Syntax.
+Require Import Logic.MinimunLogic.ProofTheory.Minimun.
+Require Import Logic.MinimunLogic.Semantics.Kripke.
+Require Logic.MinimunLogic.Complete.ContextProperty_Kripke.
+Require Import Logic.PropositionalLogic.Syntax.
+Require Logic.ModalLogic.complete.semantics.
+Require Import Logic.ModalLogic.complete.prooftheoies.
+Require Logic.ModalLogic.complete.ModalLanguage.
+Require Import Logic.ModalLogic.complete.Syntax.
+Require Import Logic.ModalLogic.complete.NormalModal.
+Local Open Scope logic_base.
+Local Open Scope syntax.
+Local Open Scope kripke_model.
+Import KripkeModelFamilyNotation.
+Import KripkeModelNotation_Intuitionistic.
+Import KripkeModelClass.
+Import ModalLanguageNotation.
+Section Canonical.
+Context {Sigma: ModalLanguage.ModalVariables}
+        {CV: Countable ModalLanguage.Var}.
+
+Existing Instances ModalLanguage.L ModalLanguage.minL ModalLanguage.pL ModalLanguage.mL.
+Existing Instances semantics.MD semantics.kMD semantics.R semantics.SM .
+
+Section General_Completeness.
+Context
+        {GammaP: Provable ModalLanguage.L}
+        {GammaD: Derivable ModalLanguage.L}.
+Definition cP : context -> Prop := Intersection _ derivable_closed consistent.
+
+Definition Relation : sig cP -> sig cP -> Prop := 
+fun Phi Psi => forall x , proj1_sig Phi (boxp x) -> proj1_sig Psi x.
+
+Definition canonical_frame: semantics.frame :=
+  semantics.Build_frame (sig cP) (fun a b => Relation a b).
+
+Definition canonical_eval: ModalLanguage.Var -> semantics.sem canonical_frame :=
+  fun p a => proj1_sig a (ModalLanguage.varp p).
+
+Definition canonical_Kmodel: @Kmodel semantics.MD semantics.kMD :=
+  semantics.Build_Kmodel canonical_frame canonical_eval.
+
+Definition rel: bijection (Kworlds canonical_Kmodel) (sig cP) := bijection_refl.
+
+Hypothesis H_R: forall m n Phi Psi, rel m Phi -> rel n Psi -> (Relation m n <-> Relation Phi Psi).
+
+Lemma Canonical_denote_ref
+  {AX: NormalAxiomatization ModalLanguage.L GammaP GammaD}
+  {SC: NormalSequentCalculus ModalLanguage.L GammaP GammaD}
+  {bSC: BasicSequentCalculus _ GammaD}
+  {minSC: MinimunSequentCalculus _ GammaD}
+  {minAX: MinimunAxiomatization ModalLanguage.L GammaP}
+  (AL_DC: at_least derivable_closed cP)
+  (AL_CONSI: at_least consistent cP)
+  (LIN_CD: forall x, Lindenbaum_constructable (cannot_derive x) cP)
+  {KmGamma : SystemK ModalLanguage.L GammaP}
+  {TmGamma :  SystemT ModalLanguage.L GammaP}:
+semantics.Krelation_ref_Kdenote (Kworlds canonical_Kmodel).
+Proof.
+  constructor.
+  intros.
+  destruct (im_bij _ _ rel w1) as [Phi ?].
+  pose proof H_R w1 w1 Phi Phi.
+  unfold KripkeModel.KM.Krelation.
+  apply H0. auto. auto.
+  hnf. intros. pose proof AL_DC.
+  hnf in H2.
+  assert(cP (proj1_sig Phi)).
+  Focus 2. apply H2 in H3 as h1.
+  pose proof derivable_closed_element_derivable (proj1_sig Phi).
+  apply H4. apply h1. assert(proj1_sig Phi |-- boxp x). apply H4. apply h1. apply H1.
+  pose proof RewriteClass.TestInSequentCalculus.Unnamed_thm (proj1_sig Phi)(boxp x) x. apply H6 in H5. apply H5.
+  apply TmGamma.
+  apply (proj2_sig Phi).
+Qed.
+Lemma Canonical_denote_trans
+  {AX: NormalAxiomatization ModalLanguage.L GammaP GammaD}
+  {SC: NormalSequentCalculus ModalLanguage.L GammaP GammaD}
+  {bSC: BasicSequentCalculus _ GammaD}
+  {minSC: MinimunSequentCalculus _ GammaD}
+  {minAX: MinimunAxiomatization ModalLanguage.L GammaP}
+  (AL_DC: at_least derivable_closed cP)
+  (AL_CONSI: at_least consistent cP)
+  (LIN_CD: forall x, Lindenbaum_constructable (cannot_derive x) cP)
+  {KmGamma : SystemK ModalLanguage.L GammaP}
+  {TmGamma : SystemT ModalLanguage.L GammaP}
+  {s4mGamma :  System4 ModalLanguage.L GammaP}:
+semantics.Krelation_trans_Kdenote (Kworlds canonical_Kmodel).
+Proof.
+  constructor.
+  intros.
+  destruct (im_bij _ _ rel w1) as [Phi1 ?].
+  destruct (im_bij _ _ rel w2) as [Phi2 ?].
+  destruct (im_bij _ _ rel w3) as [Phi3 ?].
+  pose proof H_R w1 w2 Phi1 Phi2.
+  pose proof H_R w2 w3 Phi2 Phi3.
+  pose proof H_R w1 w3 Phi1 Phi3.
+  unfold KripkeModel.KM.Krelation.
+  apply H6. auto. auto. hnf.
+  intros. pose proof AL_DC.
+  hnf in H. hnf in H0.
+  apply H4 in H1. Focus 2. auto. apply H1 in H. hnf in H.
+  apply H5 in H2. Focus 2. auto. apply H2 in H0. hnf in H0.
+  pose proof derivable_closed_element_derivable (proj1_sig Phi1).
+  pose proof derivable_closed_element_derivable (proj1_sig Phi2).
+  pose proof derivable_closed_element_derivable (proj1_sig Phi3).
+  assert (cP (proj1_sig Phi1)). Focus 2. apply H8 in H12. assert(proj1_sig Phi1 |-- boxp x). apply H9. auto. auto.
+  assert (cP (proj1_sig Phi2)). Focus 2. apply H8 in H14. assert(proj1_sig Phi2 |-- boxp x). apply H10. auto.
+  pose proof RewriteClass.TestInSequentCalculus.Unnamed_thm (proj1_sig Phi1)(boxp x) (boxp (boxp x)).
+  assert (|-- boxp x --> boxp (boxp x)). apply s4mGamma. apply H15 in H16. Focus 2. auto.
+  assert (proj1_sig Phi1 (boxp (boxp x))).
+  apply H9. auto. auto. apply H in H17. eauto. 
+  assert(proj1_sig Phi2 (boxp x)). apply H10. apply AL_DC. apply (proj2_sig Phi2).
+  auto. apply H0. auto. apply (proj2_sig Phi2). apply (proj2_sig Phi1).
+Qed.
+End General_Completeness.
+End Canonical.
